further work on completeness proof

coq/Parser_complete.v
@@ -1,8 +1,163 @@
+Require Import List.
 Require Import GallStar.Defs.
 Require Import GallStar.Lex.
 Require Import GallStar.Parser.
 Require Import GallStar.Parser_error_free.
+Require Import Prediction.
 Require Import GallStar.Tactics.
+Import ListNotations.
+
+(* a thought: maybe replace this invariant with a function of
+   the stack, i.e., "unprocessed symbols" *)
+
+Inductive tail_frames_recognize (g : grammar) : list frame -> list token -> Prop :=
+| TFR_nil :
+    tail_frames_recognize g [] []
+| TFR_cons :
+    forall o pre x suf v w w' frs,
+      gamma_recognize g suf w
+      -> tail_frames_recognize g frs w'
+      -> tail_frames_recognize g (Fr (Loc o pre (NT x :: suf)) v :: frs) (w ++ w').
+
+Hint Constructors tail_frames_recognize.
+
+Inductive stack_recognize (g : grammar) : parser_stack -> list token -> Prop :=
+| SR :
+    forall o pre suf v w w' frs,
+      gamma_recognize g suf w
+      -> tail_frames_recognize g frs w'
+      -> stack_recognize g (Fr (Loc o pre suf) v, frs) (w ++ w').
+
+Hint Constructors stack_recognize.
+
+Lemma stack_recognize_inv :
+  forall g o pre suf v frs w'',
+    stack_recognize g (Fr (Loc o pre suf) v, frs) w''
+    -> exists w w',
+      w'' = w ++ w'
+      /\ gamma_recognize g suf w
+      /\ tail_frames_recognize g frs w'.
+Proof.
+  intros g o pre suf v frs w'' hs; inv hs; eauto.
+Qed.
+
+Lemma return_preserves_stack_recognize :
+  forall g ce cr cr' frs x o o' pre pre' suf' v v' w,
+    ce = Fr (Loc o pre []) v
+    -> cr  = Fr (Loc o' pre' (NT x :: suf')) v'
+    -> cr' = Fr (Loc o' (pre' ++ [NT x]) suf') (v' ++ [Node x v])
+    -> stack_recognize g (ce, cr :: frs) w
+    -> stack_recognize g (cr', frs) w.
+Proof.
+  intros g ce cr cr' frs x o o' pre pre' suf' v v' w
+         ? ? ? hs; subst.
+  apply stack_recognize_inv in hs.
+  destruct hs as [wpre [wsuf [heq [hg ht]]]]; subst.
+  inv ht; inv hg; simpl; auto.
+Qed.
+
+Lemma gamma_recognize_terminal_head :
+  forall g a suf w,
+    gamma_recognize g (T a :: suf) w
+    -> exists l w',
+      w = (a, l) :: w'
+      /\ gamma_recognize g suf w'.
+Proof.
+  intros g a suf w hg.
+  inversion hg as [| h t wpre wsuf hs hg']; subst; clear hg.
+  inv hs; simpl; eauto.
+Qed.
+
+Lemma consume_preserves_stack_recognize :
+  forall g fr fr' frs o pre suf a l v w,
+    fr = Fr (Loc o pre (T a :: suf)) v
+    -> fr' = Fr (Loc o (pre ++ [T a]) suf) (v ++ [Leaf l])
+    -> stack_recognize g (fr, frs) ((a, l) :: w)
+    -> stack_recognize g (fr', frs) w.
+Proof.
+  intros g fr fr' frs o pre suf a l v w ? ? hs; subst.
+  apply stack_recognize_inv in hs.
+  destruct hs as [wpre [wsuf [heq [hg ht]]]]; subst.
+  apply gamma_recognize_terminal_head in hg.
+  destruct hg as [l' [w' [? hg]]]; subst.
+  inv heq; auto.
+Qed.
+
+Lemma gamma_recognize_nonterminal_head :
+  forall g x suf w,
+    gamma_recognize g (NT x :: suf) w
+    -> exists rhs wpre wsuf,
+      w = wpre ++ wsuf
+      /\ In (x, rhs) g
+      /\ gamma_recognize g rhs wpre
+      /\ gamma_recognize g suf wsuf.
+Proof.
+  intros g x suf w hg.
+  inversion hg as [| h t wpre wsuf hs hg']; subst; clear hg.
+  inv hs; simpl; eauto 8.
+Qed.
+
+Lemma push_succ_reserves_stack_derivation :
+  forall g fr o pre x suf v frs w rhs,
+    fr = Fr (Loc o pre (NT x :: suf)) v
+    -> llPredict g x (lstackOf (fr, frs)) w = PredSucc rhs
+    -> stack_recognize g (fr, frs) w
+    -> stack_recognize g (Fr (Loc (Some x) [] rhs) [], fr :: frs) w.
+Proof.
+  intros g fr o pre x suf v frs w rhs heq hl hs; subst; sis.
+  eapply stack_recognize_inv in hs.
+  destruct hs as [wpremid [wsuf [heq [hg ht]]]]; subst.
+  apply gamma_recognize_nonterminal_head in hg.
+  destruct hg as [rhs' [wpre [wmid [heq [hin [hg hg']]]]]]; subst.
+  rewrite <- app_assoc; constructor; auto.
+  eapply llPredict_succ_viable_prefix in hl; eauto.
+  - destruct hl as [vp [vs [wpre' [wsuf' [heq [heq' [hg'' [hg''' hall]]]]]]]].
+    pose proof hg as hg''''.
+    eapply hall with (viable_prefix' := rhs')
+                     (viable_suffix' := (suf ++ flat_map rsuf (map loc frs)))
+                     (wsuf' := wmid ++ wsuf) in hg; clear hall; eauto.
+    subst.
+    simpl in heq'.
+    rewrite <- app_assoc in heq'.
+    apply app_inv_head in heq'.
+    subst.
+  unfold llPredict in hl.
+  
+  
+  
+Admitted.
+
+Lemma step_preserves_stack_recognize :
+  forall g av av' stk stk' w w' u u',
+    stack_recognize g stk w
+    -> step g (Pst av stk w u) = StepK (Pst av' stk' w' u')
+    -> stack_recognize g stk' w'.
+Proof.
+  intros g av av' stk stk' w w' u u' hi hs.
+  unfold step in hs; dmeqs h; tc; inv hs; sis.
+  - eapply return_preserves_stack_recognize; eauto.
+  - eapply consume_preserves_stack_recognize; eauto.
+  - eapply push_succ_reserves_stack_derivation; eauto.
+  - admit.
+
+Inductive unprocessed_syms_recognize_suffix (g : grammar) wpre (stk : parser_stack) (w : list token) : Prop :=
+| USRS :
+    forall (wsuf : list token),
+      stack_recognize g stk wsuf
+      -> w = wpre ++ wsuf
+      -> unprocessed_syms_recognize_suffix g wpre stk w.
+    
+(* to do : prove that the above property is a parser invariant *)
+
+
+Lemma parser_doesn't_reject_valid_input :
+  forall g ys w v s,
+    gamma_derivation g ys w v
+    -> parse g ys w <> Reject s.
+Proof.
+  intros g ys w v s hg; unfold not; intros hp.
+  unfold parse in hp.
+Admitted.
 
 Lemma multistep_complete' :
   forall (g      : grammar)
@@ -38,6 +193,7 @@ Proof.
   destruct sr as [v' | s | [av' stk' wsuf' u'] | s]; subst.
   - apply step_StepAccept_facts in hs.
     destruct hs as [[o [pre [v'' [heq heq']]]] hnil]; subst.
+    unfold bottomFrameSyms in hun; simpl in hun; rewrite app_nil_r in hun.
     (* we need an invariant stating that the stack 
        captures a unique derivation *)
     admit.
@@ -64,94 +220,33 @@ Admitted.
 
 Lemma multistep_complete :
   forall (g      : grammar)
-         (tri    : nat * nat * nat)
-         (a      : Acc lex_nat_triple tri)
          (st     : parser_state)
-         (w : list token)
-         (a'     : Acc lex_nat_triple (meas g st))
-         (v      : forest),
-    tri = meas g st
-    (* you'll likely need some extra parser invariants here *)
+         (w      : list token)
+         (v      : forest)
+         (a      : Acc lex_nat_triple (meas g st)),
+    (* might need some more parser invariants here *)
+    no_left_recursion g
+    -> stack_wf g st.(stack)
+    -> unavailable_nts_invar g st
     -> unique_gamma_derivation g (bottomFrameSyms st.(stack)) w v
-    -> multistep g st a' = Accept v.
+    -> multistep g st a = Accept v.
 Proof.
-  intros.
+  intros g [av stk wsuf u] w v a hn hw hu hu'; sis.
   rewrite multistep_unfold.
   eapply multistep_complete'; eauto.
-  intros g tri a.
-  induction a as [tri hlt IH].
-  intros st w a' v ? hu; subst.
-  rewrite multistep_unfold.
-  destruct (step g st).
-Lemma multistep_complete :
-  forall (g      : grammar)
-         (tri    : nat * nat * nat)
-         (a      : Acc lex_nat_triple tri)
-         (av     : NtSet.t)
-         (stk    : parser_stack)
-         (wsuf w : list token)
-         (u      : bool)
-         (a'     : Acc lex_nat_triple (meas g (Pst av stk wsuf u)))
-         (v      : forest),
-    tri = meas g (Pst av stk wsuf u)
-    (* you'll likely need some extra parser invariants here *)
-    -> unique_gamma_derivation g (bottomFrameSyms stk) w v
-    -> multistep g (Pst av stk wsuf u) a' = Accept v.
-Proof.
-  intros g tri a.
-  induction a as [tri hlt IH].
-  intros av stk wsuf w u a' v ? hu; subst.
-  rewrite multistep_unfold.
-  pose proof (multistep_unfold_ex g (Pst av stk wsuf u) a') as hm.
-  destruct hm as [? heq'].
-  destruct x.
-  simpl in heq'.
-  destruct (step g _).
-  dmeq hs.
-  apply multistep_accept_cases.
-  unfold multistep.
-  apply multistep_accept_cases in hm.
-  destruct hm as [hf | he].
-  - apply step_StepAccept_facts in hf.
-    destruct hf as [[xo [rpre [v' [heq]]]] heq']; subst.
-    unfold bottomFrameSyms; simpl; rewrite app_nil_r.
-    eapply stack_prefix_derivation_final; eauto.
-  - destruct he as [st' [a'' [hf hm]]].
-    destruct st' as [av' stk' wsuf'].
-    eapply IH with (w := w) in hm; eauto. 
-    + erewrite step_preserves_bottomFrameSyms_invar; eauto.
-    + apply step_meas_lt; auto.
-    + eapply step_preserves_stack_wf_invar; eauto.
-    + eapply step_preserves_stack_prefix_derivation; eauto.
-  
-Lemma multistep_sound :
-  forall (g      : grammar)
-         (tri    : nat * nat * nat)
-         (a      : Acc lex_nat_triple tri)
-         (w wsuf : list token)
-         (av     : NtSet.t)
-         (stk    : parser_stack)
-         (u      : bool)
-         (a'     : Acc lex_nat_triple (meas g (Pst av stk wsuf u)))
-         (v      : forest),
-    tri = meas g (Pst av stk wsuf u)
-    -> stack_wf g stk
-    -> stack_prefix_derivation g stk wsuf w
-    -> multistep g (Pst av stk wsuf u) a' = Accept v
-    -> gamma_derivation g (bottomFrameSyms stk) w v.
-Proof.
-  
-hd : gamma_derivation g ys w v
-  hu : forall v' : forest, gamma_derivation g ys w v' -> v = v'
-  ============================
-  multistep g (mkInitState g ys w)
-    (Lex.lex_nat_triple_wf (meas g (mkInitState g ys w))) = 
-  Accept v
+Qed.
 
 Theorem parser_complete :
   forall g ys w v,
-    unique_gamma_derivation g ys w v -> parse g ys w = Accept v.
+    no_left_recursion g
+    -> unique_gamma_derivation g ys w v
+    -> parse g ys w = Accept v.
 Proof.
-  intros g ys w v [hd hu].
+  intros g ys w v hn hu.
   unfold parse.
-  
+  eapply multistep_complete with (w := w); eauto.
+  - (* lemma *)
+    constructor.
+  - apply unavailable_nts_invar_starts_true.
+Qed.
+    
